@prefix ocmv: <https://w3id.org/ontouml-models/vocabulary#> .
@prefix dcat: <http://www.w3.org/ns/dcat#> .
@prefix dct: <http://purl.org/dc/terms/> .
@prefix owl: <http://www.w3.org/2002/07/owl#> .
@prefix rdf: <http://www.w3.org/1999/02/22-rdf-syntax-ns#> .
@prefix rdfs: <http://www.w3.org/2000/01/rdf-schema#> .
@prefix skos: <http://www.w3.org/2004/02/skos/core#> .
@prefix vann: <http://purl.org/vocab/vann/> .
@prefix xml: <http://www.w3.org/XML/1998/namespace> .
@prefix xsd: <http://www.w3.org/2001/XMLSchema#> .
@prefix mod: <https://w3id.org/mod#> .

<https://w3id.org/ontouml-models/vocabulary> a owl:Ontology ;
                                             dct:title "OntoUML/UFO Catalog Metadata Vocabulary"@en ;
                                             dct:description "Metadata entities and properties to describe models in the OntoUML/UFO Catalog."@en ;
                                             dct:identifier "https://w3id.org/ontouml-models/vocabulary"^^xsd:anyURI ;
                                             dcat:landingPage <https://w3id.org/ontouml-models> ; 
                                             dcat:keyword "OntoUML"@en, "Metamodel"@en, "Ontology-Driven Conceptual Modeling"@en ;
                                             dct:creator <https://orcid.org/0000-0002-5385-5761> , 
                                                         <https://orcid.org/0000-0003-2736-7817> ,
                                                         <https://orcid.org/0000-0003-2528-3118> ,
                                                         <https://orcid.org/0000-0003-3385-4769> ;
                                             dct:isReferencedBy <https://doi.org/10.1007/978-3-031-17995-2_1> ;
                                             dct:license <https://creativecommons.org/licenses/by/4.0> ;
                                             dct:created "2022-04-03"^^xsd:date ;
                                             dct:modified "2023-03-14"^^xsd:date ;
                                             owl:versionInfo "1.0"@en ;
                                             owl:versionIRI <https://w3id.org/ontouml-models/vocabulary/1.0> ;
                                             vann:preferredNamespacePrefix "ocmv"@en ;
                                             vann:preferredNamespaceUri "https://w3id.org/ontouml-models/vocabulary#"^^xsd:anyURI .

ocmv:isComplete rdf:type owl:DatatypeProperty ;
            rdfs:label "is complete"@en ;
            rdfs:range xsd:boolean ;
            rdfs:comment "Used to indicate if a distribution is complete (i.e., containing all data) or incomplete (i.e., containing partial data)."@en .

ocmv:context a owl:ObjectProperty ;
             rdfs:label "context"@en ;
             rdfs:domain mod:SemanticArtefact ;
             rdfs:range ocmv:OntologyDevelopmentContext .

ocmv:representationStyle a owl:ObjectProperty ;
                         rdfs:label "representation style"@en ;
                         rdfs:domain mod:SemanticArtefact ;
                         rdfs:range ocmv:OntologyRepresentationStyle .

ocmv:ontologyType a owl:ObjectProperty ;
                  rdfs:label "ontology type"@en ;
                  rdfs:domain mod:SemanticArtefact ;
                  rdfs:range ocmv:OntologyType .

ocmv:conformsToSchema a owl:ObjectProperty ;
                      rdfs:label "conforms to schema"@en ;
                      rdfs:comment "Identifies a schema upon which the distribution can be validated against. E.g. a JSON Schema document, a SHACL shape, and a XML Schema document."@en ;
                      skos:scopeNote "The identified schema should be compatible with the media type of the distribution. That is, if a distribution is in JSON, the schema cannot be a SHACL shape or an XML Schema." ;
                      rdfs:domain mod:Distribution ;
                      rdfs:range rdfs:Resource .

ocmv:MetadataElement a owl:Class ;
                     rdfs:label "Metadata Element"@en ;
                     rdfs:comment "An element used in the metadata description of OntoUML models."@en .

ocmv:OntologyDevelopmentContext a owl:Class ;
                                rdfs:label "Ontology Development Context"@en ;
                                rdfs:subClassOf ocmv:MetadataElement .

ocmv:Classroom a ocmv:OntologyDevelopmentContext ;
               rdfs:label "Classroom"@en .

ocmv:Industry a ocmv:OntologyDevelopmentContext ;
              rdfs:label "Industry"@en .

ocmv:Research a ocmv:OntologyDevelopmentContext ;
              rdfs:label "Research"@en .

ocmv:OntologyPurpose a owl:Class ;
                     rdfs:label "Ontology Purpose"@en ;
                     rdfs:subClassOf ocmv:MetadataElement .

ocmv:ConceptualClarification a ocmv:OntologyPurpose ;
                             rdfs:label "Conceptual Clarification"@en .

ocmv:DataPublication a ocmv:OntologyPurpose ;
                     rdfs:label "Data Publication"@en .

ocmv:DecisionSupportSystem a ocmv:OntologyPurpose ;
                           rdfs:label "Decision Support System"@en .

ocmv:Example a ocmv:OntologyPurpose ;
             rdfs:label "Example"@en .
         
ocmv:InformationRetrieval a ocmv:OntologyPurpose ;
                          rdfs:label "Information Retrieval"@en .
         
ocmv:Interoperability a ocmv:OntologyPurpose ;
                      rdfs:label "Interoperability"@en .
         
ocmv:LanguageEngineering a ocmv:OntologyPurpose ;
                         rdfs:label "Language Engineering"@en .
         
ocmv:Learning a ocmv:OntologyPurpose ;
              rdfs:label "Learning"@en .
         
ocmv:OntologicalAnalysis a ocmv:OntologyPurpose ;
                         rdfs:label "Ontological Analysis"@en .
         
ocmv:SoftwareEngineering a ocmv:OntologyPurpose ;
                         rdfs:label "Software Engineering"@en .

ocmv:OntologyType a owl:Class ;
                  rdfs:label "Ontology Type"@en ;
                  rdfs:subClassOf ocmv:MetadataElement .

ocmv:Application a ocmv:OntologyType ;
                 rdfs:label "Application Ontology"@en .

ocmv:Core a ocmv:OntologyType ;
          rdfs:label "Core Ontology"@en .

ocmv:Domain a ocmv:OntologyType ;
            rdfs:label "Domain Ontology"@en .

ocmv:OntologyRepresentationStyle a owl:Class ;
                                 rdfs:label "Ontology Representation Style"@en ;
                                 rdfs:subClassOf ocmv:MetadataElement .

ocmv:OntoumlStyle a ocmv:OntologyRepresentationStyle ;
                  rdfs:label "OntoUML Style"@en .

ocmv:UfoStyle a ocmv:OntologyRepresentationStyle ;
              rdfs:label "UFO Style"@en .
